\begin{eqnarray}
\B_j &=& \I - \sum\limits_{i=1,i\not \in \{\ell_\mu\}}^{j-1}\beta_{ij}\GammaMat_i \B_i, \\
\C_{\ell j} &=& \beta_{\ell j} \I - \sum\limits_{i=\ell+1, i\not\in\{\ell_\mu\}}^{j-1} \beta_{\ell i}\GammaMat_i\_{\ell i}, \label{eqn:cmatdef}\\
\F_j &\equiv& \tau_{j-1} \B_{j}-\tau_{j-1} \B_{j-1}
  \ =\ - \sum\limits_{i=1,i\not \in \{\ell_\mu\}}^{j-1} \tau_{is}\GammaMat_i\B_i, \\
\G_{\ell j}&\equiv& \tau_{j-1} \C_{\ell j}-\tau_{j-1} \C_{\ell \,j-1}
  \nonumber \\
 &=&\ \tau_{\ell s}\I- \sum\limits_{i=\ell+1,i \not \in \{\ell_\mu\}}^{j-1} \tau_{is}\GammaMat_i\C_{\ell i}
\end{eqnarray}
where 